\documentclass[journal,twocolumn]{IEEEtran}
\usepackage[utf8]{inputenc}
\usepackage{amssymb}
\usepackage{amsmath}
\usepackage{graphicx}
\newcommand{\myvec}[1]{\ensuremath{\begin{pmatrix}#1\end{pmatrix}}}
\providecommand{\brak}[1]{\ensuremath{\left(#1\right)}}
\title{Assignment 6}
\author{NIMMALA AVINASH(CS21BTECH11039)}
\begin{document}

\maketitle

{\LARGE \textbf{Question:\\}}
Suppose $ x $ and $ y $ have joint density
\begin{align}
f_{xy}(x,y)=\begin{cases}
1 &0\leq x\leq 2,0\leq y\leq 1,2y \leq x\\
0 &otherwise
\end{cases}
\end{align}
show that $ z = x+y $ has density
\begin{align}
f_{xy}(x,y) = \begin{cases}
(1/3)z &0\leq z\leq 2\\
2-(2/3)z &2\leq z\leq 3\\
0 &elsewhere
\end{cases}
\end{align}
{\LARGE \textbf{Solution:}}
\begin{align}
F_{Z}(z) &= P(X+Y \leq z)\\
&=\begin{cases}
P(X+Y\leq z), &0 < z < 2\\
1-P(X+Y>z), &2 < z < 3\\
\end{cases}\\
where,\\
 &2y\leq x ,\implies3y\leq x+y \implies y \leq \frac{z}{3}\\
 & 2y \leq x \leq z-y\\
 & 0 \leq y \leq \frac{z}{3}\\
&=\begin{cases}
\int_{0}^{z/3} \int_{2y}^{z-y}f_{XY}(x,y) dx dy  , &0 < z < 2\\
1-\int_{2z/3}^{2} \int_{z-x}^{x/2}f_{XY}(x,y) dy dx , &2 < z < 3\\
\end{cases}\\
&=\begin{cases}
\int_{0}^{z/3}(z-3y)dy , &0 < z < 2\\
1-\int_{2z/3}^{2}(\frac{3x}{2}-z)dx &2 < z < 3\\
\end{cases}\\
&=\begin{cases}
\frac{z^{2}}{6}, &0 < z < 2\\
2z-\frac{z^{2}}{3}-2,&2 < z < 3\\
\end{cases}
\end{align}
Thus\\
\begin{align}
f_{Z}(z)&=\frac{d}{dz}(F_{Z}(z))\\
f_{Z}(z)&=\begin{cases}
\frac{1}{3}z,&0 < z < 2\\
2-\frac{2z}{3},&2 < z < 3\\
0,&otherwise
\end{cases}
\end{align}
\end{document}